src/lib/kernel/gemm/Kuiper.Kernel.GEMM.TensorCore2D.To.Epilogue.fst
@@ -1,0 +1,626 @@
+module Kuiper.Kernel.GEMM.TensorCore2D.To.Epilogue
+
+#lang-pulse
+
+open Kuiper
+#set-options "--ifuel 1 --initial_fuel 0 --max_fuel 1"
+#set-options "--z3rlimit 120"
+
+open Kuiper.Array.Vectorized { has_vec_cpy, chunk }
+open Kuiper.EMatrix
+open Kuiper.Float16
+open Kuiper.Math { even, odd, even_2x, odd_2x1 }
+open Kuiper.Tensor
+open Kuiper.Array2.Strided
+open Kuiper.Tensor.Tiling
+open Kuiper.Tensor.Layout.Alg { l2_row_major as rm }
+open Kuiper.Kernel.GEMM.Copy.Vec2
+open Kuiper.Kernel.GEMM.Tiled.Common.Vec
+open Kuiper.Spec.GEMM
+open Kuiper.TensorCore
+open Pulse.Lib.Array
+open Pulse.Lib.Trade
+
+module SZ = Kuiper.SizeT
+module B = Kuiper.Barrier
+module T = Kuiper.Tensor
+module FB = Kuiper.Kernel.GEMM.FlipFlopBarrier2
+module CV2 = Kuiper.Kernel.GEMM.Copy.Vec2
+module BW = Kuiper.Barrier.Warp
+
+open Kuiper.Kernel.GEMM.TensorCore2D.KernelDesc
+
+
+open Kuiper.Kernel.GEMM.TensorCore2D.To.KernelDesc
+
+let output_fragment_post
+  (#et : Type0) {| scalar et, real_like et |}
+  (#m #n : nat)
+  (gD : array2 et (rm m n))
+  (bm bn tm tn wm wn : pos)
+  (#_ : squash (bm /?+ m /\ bn /?+ n /\
+                wm * tm /?+ bm /\ wn * tn /?+ bn))
+  (bid : natlt (m / bm * (n / bn)))
+  (wid : natlt (bm / (wm * tm) * (bn / (wn * tn))))
+  (lane : natlt warp_size)
+  (rD : chest2 real (wm * tm) (wn * tn))
+  (idx : natlt (wm * wn))
+  : slprop
+= exists* (eD : chest2 et tm tn).
+    own_lane_cells
+      (output_fragment gD bm bn tm tn wm wn
+        bid wid (idx / wn) (idx % wn))
+      eD lane **
+    pure (eD %~ ematrix_subtile rD tm tn (idx / wn) (idx % wn))
+
+let if_else_ (b : bool) (p q : slprop) : slprop =
+  if_ b p ** if_ (not b) q
+
+ghost
+fn warp_emp_transform ()
+  requires forall+ (_ : natlt BW.warp_size). emp
+  ensures forall+ (_ : natlt BW.warp_size). emp
+{}
+
+  ghost
+  fn forevery_extract_replace_eqtype
+    (#a : eqtype)
+    (z : a)
+    (p1 p2 : a -> slprop)
+    (#_ : squash (forall x. x =!= z ==> p1 x == p2 x))
+    requires forall+ (x : a). p1 x
+    ensures
+      p1 z **
+      (p2 z @==> forall+ (x : a). p2 x)
+  {
+    forevery_extract_if_eqtype z p1;
+    intro_trade #emp_inames
+      (p2 z)
+      (forall+ (x : a). p2 x)
+      (forall+ (x : a). if x = z then emp else p1 x)
+      fn _ {
+        forevery_map #a
+          (fun x -> if x = z then emp else p1 x)
+          (fun x -> if x = z then emp else p2 x)
+          fn x {
+            let is_z = x = z;
+            if is_z {
+              rewrite
+                (if x = z then emp else p1 x)
+              as emp;
+              rewrite emp as
+                (if x = z then emp else p2 x);
+            } else {
+              rewrite
+                (if x = z then emp else p1 x)
+              as p1 x;
+              rewrite p1 x as p2 x;
+              rewrite p2 x as
+                (if x = z then emp else p2 x);
+            }
+          };
+        forevery_unextract_if_eqtype z p2;
+      };
+  }
+
+  ghost
+  fn forevery_insert_replace_eqtype
+    (#a : eqtype)
+    (z : a)
+    (p1 p2 : a -> slprop)
+    (#_ : squash (forall x. x =!= z ==> p1 x == p2 x))
+    requires
+      p2 z **
+      (forall+ (x : a { x =!= z }). p1 x)
+    ensures forall+ (x : a). p2 x
+  {
+    forevery_map
+      #(x : a { x =!= z })
+      p1 p2
+      fn x {
+        rewrite p1 x as p2 x;
+      };
+    forevery_insert
+      #a
+      #(fun x -> x =!= z)
+      p2 z;
+    forevery_refine_ext
+      #a
+      #(fun x -> x =!= z \/ z == x)
+      (fun _ -> True)
+      p2;
+  }
+
+  let output_fragment_state_at
+    (#et : Type0) {| scalar et, real_like et |}
+    (#m #n : nat)
+    (gD : array2 et (rm m n))
+    (bm bn tm tn wm wn : pos)
+    (#_ : squash (bm /?+ m /\ bn /?+ n /\
+                  wm * tm /?+ bm /\ wn * tn /?+ bn))
+    (bid : natlt (m / bm * (n / bn)))
+    (wid : natlt (bm / (wm * tm) * (bn / (wn * tn))))
+    (lane : natlt warp_size)
+    (rD : chest2 real (wm * tm) (wn * tn))
+    (done : natle (wm * wn))
+    (idx : natlt (wm * wn))
+    : slprop
+  = if_else_ (idx < done)
+      (output_fragment_post
+        gD bm bn tm tn wm wn bid wid lane rD idx)
+      (live_lane_cells
+        (output_fragment gD bm bn tm tn wm wn
+          bid wid (idx / wn) (idx % wn))
+        lane)
+
+  let output_epilogue_state
+  (#et : Type0) {| scalar et, real_like et |}
+  (#m #n : nat)
+  (gD : array2 et (rm m n))
+  (bm bn tm tn wm wn : pos)
+  (#_ : squash (bm /?+ m /\ bn /?+ n /\
+                wm * tm /?+ bm /\ wn * tn /?+ bn))
+  (bid : natlt (m / bm * (n / bn)))
+  (wid : natlt (bm / (wm * tm) * (bn / (wn * tn))))
+  (lane : natlt warp_size)
+  (rD : chest2 real (wm * tm) (wn * tn))
+  (done : natle (wm * wn))
+  : slprop
+= forall+ (idx : natlt (wm * wn)).
+    output_fragment_state_at
+      gD bm bn tm tn wm wn bid wid lane rD done idx
+
+ghost
+fn output_epilogue_extract_step
+  (#et : Type0) {| scalar et, real_like et |}
+  (#m #n : nat)
+  (gD : array2 et (rm m n))
+  (bm bn tm tn wm wn : pos)
+  (#_ : squash (bm /?+ m /\ bn /?+ n /\
+                wm * tm /?+ bm /\ wn * tn /?+ bn))
+  (bid : natlt (m / bm * (n / bn)))
+  (wid : natlt (bm / (wm * tm) * (bn / (wn * tn))))
+  (lane : natlt warp_size)
+  (rD : chest2 real (wm * tm) (wn * tn))
+  (idx_ref : ref (szle (wm * wn)))
+  (done : szle (wm * wn) { SZ.v done < wm * wn })
+  preserves idx_ref |-> done
+  requires
+    output_epilogue_state
+      gD bm bn tm tn wm wn bid wid lane rD (SZ.v done)
+  ensures
+    output_fragment_state_at
+      gD bm bn tm tn wm wn bid wid lane rD
+      (SZ.v done) (SZ.v done) **
+    (output_fragment_state_at
+        gD bm bn tm tn wm wn bid wid lane rD
+        (SZ.v done + 1) (SZ.v done)
+      @==>
+      forall+ (idx : natlt (wm * wn)).
+        output_fragment_state_at
+          gD bm bn tm tn wm wn bid wid lane rD (SZ.v done + 1) idx)
+{
+  unfold output_epilogue_state
+    gD bm bn tm tn wm wn bid wid lane rD (SZ.v done);
+  forevery_extract_replace_eqtype
+    #(natlt (wm * wn))
+    (SZ.v done)
+    (output_fragment_state_at
+      gD bm bn tm tn wm wn bid wid lane rD (SZ.v done))
+    (output_fragment_state_at
+      gD bm bn tm tn wm wn bid wid lane rD (SZ.v done + 1));
+}
+
+inline_for_extraction noextract
+fn epilogue_to
+  (#et_ab #et_cd #et_acc : Type0)
+  {| scalar et_ab, scalar et_cd, real_like et_cd,
+     scalar et_acc, real_like et_acc |}
+  (comb : et_cd -> et_acc -> et_cd)
+  (comb_r : binop real { approx2 comb comb_r })
+  (#m #n : szp)
+  (gC : array2 et_cd (rm m n))
+  (#fC : perm)
+  (#eC : chest2 et_cd m n)
+  (#rC : chest2 real m n)
+  (#_ : squash (eC %~ rC))
+  (gD : array2 et_cd (rm m n))
+  (#_ : squash (SZ.fits (m * n)))
+  (bm bn bk tm tn tk wm wn nthr : szp{
+    constraints bm bn bk tm tn tk wm wn /\
+    SZ.v nthr == bm / (wm * tm) * (bn / (wn * tn)) * warp_size})
+  (#_ : squash (bm /?+ m /\ bn /?+ n))
+  (#_ : squash (SZ.fits (bm * bk) /\ SZ.fits (bk * bn)))
+  (#_ : squash (SZ.fits (wm * wn)))
+  (#_ : squash (SZ.fits ((nthr / warp_size) * tm * tn)))
+  (#_ : squash (SZ.fits (tm * tn + warp_size)))
+  (sh : c_shmems (shmems_desc_to et_ab et_acc bm bn bk tm tn nthr))
+  (accFrags : array (fragment et_acc FragAcc tm tn tk FragLAcc))
+  (rAcc : chest2 real (wm * tm) (wn * tn))
+  (bid : szlt (m / bm * (n / bn)))
+  (tid : szlt nthr)
+  (#_ : squash (Pulse.Lib.Array.length accFrags == wm * wn))
+  preserves
+    gpu **
+    thread_id nthr tid **
+    gC |-> Frac fC eC **
+    fragarrayAcc_approximates wm wn accFrags rAcc
+  requires
+    scratch_tile_live bm bn bk tm tn nthr sh tid **
+    output_lane_live gD bm bn tm tn wm wn bid tid
+  ensures
+    scratch_tile_live bm bn bk tm tn nthr sh tid **
+    output_lane_approximates
+      gD bm bn tm tn wm wn bid tid
+      (chest_comb comb_r
+        (ematrix_subtile
+          (ematrix_subtile rC bm bn
+            (bid / (n / bn)) (bid % (n / bn)))
+          (wm * tm) (wn * tn)
+          ((tid / warp_size) / (bn / (wn * tn)))
+          ((tid / warp_size) % (bn / (wn * tn))))
+        rAcc)
+{
+  let wid = tid /^ warp_size;
+  let lane = tid %^ warp_size;
+  let mrow = bid /^ (n /^ bn);
+  let mcol = bid %^ (n /^ bn);
+  let warpRow = wid /^ (bn /^ (wn *^ tn));
+  let warpCol = wid %^ (bn /^ (wn *^ tn));
+  let rCWarp =
+    ematrix_subtile
+      (ematrix_subtile rC bm bn mrow mcol)
+      (wm * tm) (wn * tn) warpRow warpCol;
+
+  unfold output_lane_live gD bm bn tm tn wm wn bid tid;
+  forevery_flatten _;
+  forevery_iso
+    (Kuiper.Bijection.bij_nat_prod #wm #wn)
+    (fun (xy : (natlt wm & natlt wn)) ->
+      live_lane_cells
+        (output_fragment gD bm bn tm tn wm wn
+          bid (tid / warp_size) xy._1 xy._2)
+        (tid % warp_size));
+  rewrite each (tid / warp_size) as wid;
+  rewrite each (tid % warp_size) as lane;
+  let output_live =
+    (fun (idx : natlt (wm * wn)) ->
+      live_lane_cells
+        (output_fragment gD bm bn tm tn wm wn
+          bid wid (idx / wn) (idx % wn))
+        lane);
+  forevery_ext
+    (fun (idx : natlt (wm * wn)) ->
+      live_lane_cells
+        (output_fragment gD bm bn tm tn wm wn
+          bid wid (idx / wn) (idx % wn))
+        lane)
+    output_live;
+  forevery_map
+    #(natlt (wm * wn))
+    output_live
+    (fun idx ->
+      output_fragment_state_at
+        gD bm bn tm tn wm wn bid wid lane
+        (chest_comb comb_r rCWarp rAcc) 0 idx)
+    fn idx {
+      rewrite output_live idx as
+        live_lane_cells
+          (output_fragment gD bm bn tm tn wm wn
+            bid wid (idx / wn) (idx % wn))
+          lane;
+      Kuiper.Conditional.if_intro_false
+        (output_fragment_post
+          gD bm bn tm tn wm wn bid wid lane
+          (chest_comb comb_r rCWarp rAcc) idx);
+      Kuiper.Conditional.if_rewrite_bool
+        false (idx < 0)
+        (output_fragment_post
+          gD bm bn tm tn wm wn bid wid lane
+          (chest_comb comb_r rCWarp rAcc) idx);
+      Kuiper.Conditional.if_intro_true
+        (live_lane_cells
+          (output_fragment gD bm bn tm tn wm wn
+            bid wid (idx / wn) (idx % wn))
+          lane);
+      Kuiper.Conditional.if_rewrite_bool
+        true (not (idx < 0))
+        (live_lane_cells
+          (output_fragment gD bm bn tm tn wm wn
+            bid wid (idx / wn) (idx % wn))
+          lane);
+      fold if_else_ (idx < 0)
+        (output_fragment_post
+          gD bm bn tm tn wm wn bid wid lane
+          (chest_comb comb_r rCWarp rAcc) idx)
+        (live_lane_cells
+          (output_fragment gD bm bn tm tn wm wn
+            bid wid (idx / wn) (idx % wn))
+          lane);
+      fold output_fragment_state_at
+        gD bm bn tm tn wm wn bid wid lane
+        (chest_comb comb_r rCWarp rAcc) 0 idx;
+    };
+  fold output_epilogue_state
+    gD bm bn tm tn wm wn bid wid lane
+    (chest_comb comb_r rCWarp rAcc) 0;
+
+  with eScratch.
+    unfold scratch_tile_live bm bn bk tm tn nthr sh tid;
+  let sTile = scratch_tile_st bm bn bk tm tn nthr sh wid;
+
+  let mut idx : szle (wm * wn) = 0sz;
+  while (!idx <^ wm *^ wn)
+    invariant live idx
+    invariant
+      exists* (eScratchLoop : chest2 et_acc tm tn).
+        scratch_tile bm bn bk tm tn nthr sh
+          (SZ.v tid / warp_size)
+          |-> Frac (1.0R /. warp_size) eScratchLoop
+    invariant
+      output_epilogue_state
+        gD bm bn tm tn wm wn bid wid lane
+        (chest_comb comb_r rCWarp rAcc) !idx
+    invariant
+      fragarrayAcc_approximates wm wn accFrags rAcc
+    decreases (wm * wn - !idx)
+  {
+    with vidx. assert idx |-> vidx;
+    output_epilogue_extract_step
+      gD bm bn tm tn wm wn bid wid lane
+      (chest_comb comb_r rCWarp rAcc) idx vidx;
+    unfold output_fragment_state_at
+      gD bm bn tm tn wm wn bid wid lane
+      (chest_comb comb_r rCWarp rAcc) (SZ.v vidx) (SZ.v vidx);
+    unfold if_else_ (SZ.v vidx < SZ.v vidx)
+      (output_fragment_post
+        gD bm bn tm tn wm wn bid wid lane
+        (chest_comb comb_r rCWarp rAcc) (SZ.v vidx))
+      (live_lane_cells
+        (output_fragment gD bm bn tm tn wm wn
+          bid wid (SZ.v vidx / wn) (SZ.v vidx % wn))
+        lane);
+    Kuiper.Conditional.if_rewrite_bool
+      (SZ.v vidx < SZ.v vidx) false
+      (output_fragment_post
+        gD bm bn tm tn wm wn bid wid lane
+        (chest_comb comb_r rCWarp rAcc) (SZ.v vidx));
+    Kuiper.Conditional.if_elim_false
+      (output_fragment_post
+        gD bm bn tm tn wm wn bid wid lane
+        (chest_comb comb_r rCWarp rAcc) (SZ.v vidx));
+    Kuiper.Conditional.if_rewrite_bool
+      (not (SZ.v vidx < SZ.v vidx)) true
+      (live_lane_cells
+        (output_fragment gD bm bn tm tn wm wn
+          bid wid (SZ.v vidx / wn) (SZ.v vidx % wn))
+        lane);
+    Kuiper.Conditional.if_elim_true
+      (live_lane_cells
+        (output_fragment gD bm bn tm tn wm wn
+          bid wid (SZ.v vidx / wn) (SZ.v vidx % wn))
+        lane);
+
+    unfold fragarrayAcc_approximates wm wn accFrags rAcc;
+    with eAccFrags. assert accFrags `array_fragment_pts_to` eAccFrags;
+    array_fragment_pts_to_ref accFrags;
+    array_fragment_extract_ro accFrags vidx;
+
+    rewrite each
+      scratch_tile bm bn bk tm tn nthr sh (SZ.v tid / warp_size)
+    as sTile;
+    mma_store accFrags.(!idx) sTile;
+
+    BW.warp_barrier_wait ()
+      (fun _ -> emp)
+      (fun _ -> emp)
+      warp_emp_transform;
+
+    let rCFrag =
+      ematrix_subtile rCWarp tm tn (SZ.v vidx / wn) (SZ.v vidx % wn);
+    let rAccFrag =
+      ematrix_subtile rAcc tm tn (SZ.v vidx / wn) (SZ.v vidx % wn);
+
+    assert pure (Seq.Base.index eAccFrags vidx %~ rAccFrag);
+    epilogue_fragment_from_warp comb comb_r gC
+      bm bn tm tn wm wn mrow mcol warpRow warpCol bid wid
+      #_ #_ #_ #rC #_
+      sTile #(Seq.Base.index eAccFrags vidx) #rAccFrag #_
+      gD !idx lane;
+    rewrite each sTile as
+      scratch_tile bm bn bk tm tn nthr sh (SZ.v tid / warp_size);
+
+    with eOut.
+      assert own_lane_cells
+        (output_fragment gD bm bn tm tn wm wn
+          bid wid (SZ.v vidx / wn) (SZ.v vidx % wn))
+        eOut lane;
+    fold output_fragment_post
+      gD bm bn tm tn wm wn bid wid lane
+      (chest_comb comb_r rCWarp rAcc) vidx;
+    Kuiper.Conditional.if_intro_true
+      (output_fragment_post
+        gD bm bn tm tn wm wn bid wid lane
+        (chest_comb comb_r rCWarp rAcc) (SZ.v vidx));
+    Kuiper.Conditional.if_rewrite_bool
+      true (SZ.v vidx < SZ.v vidx + 1)
+      (output_fragment_post
+        gD bm bn tm tn wm wn bid wid lane
+        (chest_comb comb_r rCWarp rAcc) (SZ.v vidx));
+    Kuiper.Conditional.if_intro_false
+      (live_lane_cells
+        (output_fragment gD bm bn tm tn wm wn
+          bid wid (SZ.v vidx / wn) (SZ.v vidx % wn))
+        lane);
+    Kuiper.Conditional.if_rewrite_bool
+      false (not (SZ.v vidx < SZ.v vidx + 1))
+      (live_lane_cells
+        (output_fragment gD bm bn tm tn wm wn
+          bid wid (SZ.v vidx / wn) (SZ.v vidx % wn))
+        lane);
+    fold if_else_ (SZ.v vidx < SZ.v vidx + 1)
+      (output_fragment_post
+        gD bm bn tm tn wm wn bid wid lane
+        (chest_comb comb_r rCWarp rAcc) (SZ.v vidx))
+      (live_lane_cells
+        (output_fragment gD bm bn tm tn wm wn
+          bid wid (SZ.v vidx / wn) (SZ.v vidx % wn))
+        lane);
+    fold output_fragment_state_at
+      gD bm bn tm tn wm wn bid wid lane
+      (chest_comb comb_r rCWarp rAcc)
+      (SZ.v vidx + 1) (SZ.v vidx);
+    Pulse.Lib.Trade.elim_trade
+      (output_fragment_state_at
+        gD bm bn tm tn wm wn bid wid lane
+        (chest_comb comb_r rCWarp rAcc)
+        (SZ.v vidx + 1) (SZ.v vidx))
+      (forall+ (fi : natlt (wm * wn)).
+        output_fragment_state_at
+          gD bm bn tm tn wm wn bid wid lane
+          (chest_comb comb_r rCWarp rAcc) (SZ.v vidx + 1) fi);
+    ambig_trade_elim ();
+    fold fragarrayAcc_approximates wm wn accFrags rAcc;
+
+    fold output_epilogue_state
+      gD bm bn tm tn wm wn bid wid lane
+      (chest_comb comb_r rCWarp rAcc) (SZ.v vidx + 1);
+    with vnext. assert idx |-> vnext;
+    idx := sz_succ !idx;
+    rewrite each
+      (SZ.v vnext + 1)
+    as
+      (SZ.v (sz_succ vnext));
+  };
+
+  rewrite each !idx as (wm *^ wn);
+  fold scratch_tile_live bm bn bk tm tn nthr sh tid;
+  unfold output_epilogue_state
+    gD bm bn tm tn wm wn bid wid lane
+    (chest_comb comb_r rCWarp rAcc) (wm * wn);
+  forevery_map
+    #(natlt (wm * wn))
+    (fun (fi : natlt (wm * wn)) ->
+      output_fragment_state_at
+        gD bm bn tm tn wm wn bid wid lane
+        (chest_comb comb_r rCWarp rAcc) (wm * wn) fi)
+    (fun (fi : natlt (wm * wn)) ->
+      output_fragment_post
+        gD bm bn tm tn wm wn bid wid lane
+        (chest_comb comb_r rCWarp rAcc) fi)
+    fn fi {
+      unfold output_fragment_state_at
+        gD bm bn tm tn wm wn bid wid lane
+        (chest_comb comb_r rCWarp rAcc) (wm * wn) fi;
+      unfold if_else_ (fi < wm * wn)
+        (output_fragment_post
+          gD bm bn tm tn wm wn bid wid lane
+          (chest_comb comb_r rCWarp rAcc) fi)
+        (live_lane_cells
+          (output_fragment gD bm bn tm tn wm wn
+            bid wid (fi / wn) (fi % wn))
+          lane);
+      Kuiper.Conditional.if_rewrite_bool
+        (fi < wm * wn) true
+        (output_fragment_post
+          gD bm bn tm tn wm wn bid wid lane
+          (chest_comb comb_r rCWarp rAcc) fi);
+      Kuiper.Conditional.if_elim_true
+        (output_fragment_post
+          gD bm bn tm tn wm wn bid wid lane
+          (chest_comb comb_r rCWarp rAcc) fi);
+      Kuiper.Conditional.if_rewrite_bool
+        (not (fi < wm * wn)) false
+        (live_lane_cells
+          (output_fragment gD bm bn tm tn wm wn
+            bid wid (fi / wn) (fi % wn))
+          lane);
+      Kuiper.Conditional.if_elim_false
+        (live_lane_cells
+          (output_fragment gD bm bn tm tn wm wn
+            bid wid (fi / wn) (fi % wn))
+          lane);
+    };
+  forevery_ext
+    (fun (fi : natlt (wm * wn)) ->
+      output_fragment_post
+        gD bm bn tm tn wm wn bid wid lane
+        (chest_comb comb_r rCWarp rAcc) fi)
+    (fun (fi : natlt (wm * wn)) ->
+      output_fragment_post
+        gD bm bn tm tn wm wn bid wid lane
+        (chest_comb comb_r rCWarp rAcc)
+        (fi / wn * wn + fi % wn));
+  forevery_iso_back
+    (Kuiper.Bijection.bij_nat_prod #wm #wn)
+    (fun xy ->
+      output_fragment_post
+        gD bm bn tm tn wm wn bid wid lane
+        (chest_comb comb_r rCWarp rAcc)
+        (xy._1 * wn + xy._2));
+  forevery_map
+    #(natlt wm & natlt wn)
+    (fun (xy : (natlt wm & natlt wn)) ->
+      output_fragment_post
+        gD bm bn tm tn wm wn bid wid lane
+        (chest_comb comb_r rCWarp rAcc)
+        (xy._1 * wn + xy._2))
+    (fun (xy : (natlt wm & natlt wn)) ->
+      exists* (eD : chest2 et_cd tm tn).
+        own_lane_cells
+          (output_fragment gD bm bn tm tn wm wn
+            bid wid xy._1 xy._2)
+          eD lane **
+        pure (eD %~
+          ematrix_subtile
+            (chest_comb comb_r rCWarp rAcc)
+            tm tn xy._1 xy._2))
+    fn xy {
+      unfold output_fragment_post
+        gD bm bn tm tn wm wn bid wid lane
+        (chest_comb comb_r rCWarp rAcc)
+        (xy._1 * wn + xy._2);
+      assert pure (
+        (xy._1 * wn + xy._2) / wn == xy._1);
+      assert pure (
+        (xy._1 * wn + xy._2) % wn == xy._2);
+      rewrite each
+        ((xy._1 * wn + xy._2) / wn)
+      as xy._1;
+      rewrite each
+        ((xy._1 * wn + xy._2) % wn)
+      as xy._2;
+    };
+  forevery_unflatten
+    (fun (mi : natlt wm) (nj : natlt wn) ->
+      exists* (eD : chest2 et_cd tm tn).
+        own_lane_cells
+          (output_fragment gD bm bn tm tn wm wn bid wid mi nj)
+          eD lane **
+        pure (eD %~
+          ematrix_subtile
+            (chest_comb comb_r rCWarp rAcc)
+            tm tn mi nj));
+  rewrite each rCWarp as
+    ematrix_subtile
+      (ematrix_subtile rC bm bn mrow mcol)
+      (wm * tm) (wn * tn) warpRow warpCol;
+  rewrite each (SZ.v mrow) as (SZ.v bid / (SZ.v n / SZ.v bn));
+  rewrite each (SZ.v mcol) as (SZ.v bid % (SZ.v n / SZ.v bn));
+  rewrite each (SZ.v warpRow) as
+    ((SZ.v tid / warp_size) / (SZ.v bn / (SZ.v wn * SZ.v tn)));
+  rewrite each (SZ.v warpCol) as
+    ((SZ.v tid / warp_size) % (SZ.v bn / (SZ.v wn * SZ.v tn)));
+  rewrite each (SZ.v wid) as (SZ.v tid / warp_size);
+  rewrite each (SZ.v lane) as (SZ.v tid % warp_size);
+  fold output_lane_approximates
+    gD bm bn tm tn wm wn bid tid
+    (chest_comb comb_r
+      (ematrix_subtile
+        (ematrix_subtile rC bm bn
+          (bid / (n / bn)) (bid % (n / bn)))
+        (wm * tm) (wn * tn)
+        ((tid / warp_size) / (bn / (wn * tn)))
+        ((tid / warp_size) % (bn / (wn * tn))))
+      rAcc);
+}
