src/lib/kernel/gemm/Kuiper.Kernel.GEMM.TensorCore2D.To.Epilogue.fsti
@@ -1,0 +1,85 @@
+module Kuiper.Kernel.GEMM.TensorCore2D.To.Epilogue
+
+#lang-pulse
+
+open Kuiper
+open Kuiper.EMatrix
+open Kuiper.EMatrix.Tiling
+open Kuiper.Tensor
+open Kuiper.Tensor.Layout.Alg { l2_row_major as rm }
+open Kuiper.TensorCore
+open Pulse.Lib.Array
+
+module SZ = Kuiper.SizeT
+
+open Kuiper.Kernel.GEMM.TensorCore2D.KernelDesc
+open Kuiper.Kernel.GEMM.TensorCore2D.To.KernelDesc
+
+inline_for_extraction noextract
+let sz_succ (x : SZ.t { SZ.fits (x + 1) }) : SZ.t = x +^ 1sz
+
+let fragarrayAcc_approximates
+  (#et:Type0) {| scalar et, real_like et |}
+  (#tm #tn #tk : pos)
+  (wm wn : nat)
+  ([@@@mkey] arr : array (fragment et FragAcc tm tn tk FragLAcc) {
+    Pulse.Lib.Array.length arr == wm * wn})
+  (rm : chest2 real (wm * tm) (wn * tn))
+  : slprop
+= exists* (em : seq (chest2 et tm tn)).
+    arr |-> em **
+    pure (
+      Seq.length em == wm * wn /\
+      forall (i : natlt wm) (j : natlt wn).
+        Seq.index em (i * wn + j) %~
+          ematrix_subtile rm tm tn i j)
+
+inline_for_extraction noextract
+fn epilogue_to
+  (#et_ab #et_cd #et_acc : Type0)
+  {| scalar et_ab, scalar et_cd, real_like et_cd,
+     scalar et_acc, real_like et_acc |}
+  (comb : et_cd -> et_acc -> et_cd)
+  (comb_r : binop real { approx2 comb comb_r })
+  (#m #n : szp)
+  (gC : array2 et_cd (rm m n))
+  (#fC : perm)
+  (#eC : chest2 et_cd m n)
+  (#rC : chest2 real m n)
+  (#_ : squash (eC %~ rC))
+  (gD : array2 et_cd (rm m n))
+  (#_ : squash (SZ.fits (m * n)))
+  (bm bn bk tm tn tk wm wn nthr : szp{
+    constraints bm bn bk tm tn tk wm wn /\
+    SZ.v nthr == bm / (wm * tm) * (bn / (wn * tn)) * warp_size})
+  (#_ : squash (bm /?+ m /\ bn /?+ n))
+  (#_ : squash (SZ.fits (bm * bk) /\ SZ.fits (bk * bn)))
+  (#_ : squash (SZ.fits (wm * wn)))
+  (#_ : squash (SZ.fits ((nthr / warp_size) * tm * tn)))
+  (#_ : squash (SZ.fits (tm * tn + warp_size)))
+  (sh : c_shmems (shmems_desc_to et_ab et_acc bm bn bk tm tn nthr))
+  (accFrags : array (fragment et_acc FragAcc tm tn tk FragLAcc))
+  (rAcc : chest2 real (wm * tm) (wn * tn))
+  (bid : szlt (m / bm * (n / bn)))
+  (tid : szlt nthr)
+  (#_ : squash (Pulse.Lib.Array.length accFrags == wm * wn))
+  preserves
+    gpu **
+    thread_id nthr tid **
+    gC |-> Frac fC eC **
+    fragarrayAcc_approximates wm wn accFrags rAcc
+  requires
+    scratch_tile_live bm bn bk tm tn nthr sh tid **
+    output_lane_live gD bm bn tm tn wm wn bid tid
+  ensures
+    scratch_tile_live bm bn bk tm tn nthr sh tid **
+    output_lane_approximates
+      gD bm bn tm tn wm wn bid tid
+      (chest_comb comb_r
+        (ematrix_subtile
+          (ematrix_subtile rC bm bn
+            (bid / (n / bn)) (bid % (n / bn)))
+          (wm * tm) (wn * tn)
+          ((tid / warp_size) / (bn / (wn * tn)))
+          ((tid / warp_size) % (bn / (wn * tn))))
+        rAcc)
