src/lib/kernel/gemm/Kuiper.Kernel.GEMM.TensorCore2D.To.KernelDesc.fsti
@@ -1,0 +1,607 @@
+module Kuiper.Kernel.GEMM.TensorCore2D.To.KernelDesc
+
+#lang-pulse
+
+open Kuiper
+open Kuiper.Array.Vectorized { has_vec_cpy, chunk }
+open Kuiper.EMatrix
+open Kuiper.Tensor
+open Kuiper.Array2.Strided
+open Kuiper.Tensor.Tiling
+open Kuiper.Tensor.Layout.Alg { l2_row_major as rm }
+open Kuiper.Kernel.GEMM.Tiled.Common.Vec
+open Kuiper.TensorCore
+
+module SZ = Kuiper.SizeT
+module T = Kuiper.Tensor
+module MS = Kuiper.Spec.GEMM
+
+open Kuiper.Kernel.GEMM.TensorCore2D.KernelDesc
+
+let in_lane
+  (rows cols : nat)
+  (lane : natlt warp_size)
+  (ij : natlt rows & natlt cols)
+  : prop
+= (ij._1 * cols + ij._2) % warp_size == lane
+
+let own_lane_cells
+  (#et : Type0) {| scalar et |}
+  (#rows #cols : nat)
+  (#l : layout2 rows cols)
+  ([@@@mkey] m : array2 et l)
+  (em : chest2 et rows cols)
+  (lane : natlt warp_size)
+  : slprop
+= forall+ (ij : (natlt rows & natlt cols){in_lane rows cols lane ij}).
+    tensor_pts_to_cell m (idx2 ij._1 ij._2) (acc2 em ij._1 ij._2)
+
+let live_lane_cells
+  (#et : Type0) {| scalar et |}
+  (#rows #cols : nat)
+  (#l : layout2 rows cols)
+  ([@@@mkey] m : array2 et l)
+  (lane : natlt warp_size)
+  : slprop
+= exists* (em : chest2 et rows cols). own_lane_cells m em lane
+
+inline_for_extraction noextract
+let output_fragment
+  (#et : Type0) {| scalar et |}
+  (#m #n : nat)
+  (gD : array2 et (rm m n))
+  (bm bn tm tn wm wn : pos)
+  (#_ : squash (bm /?+ m /\ bn /?+ n /\
+                wm * tm /?+ bm /\ wn * tn /?+ bn))
+  (bid : natlt (m / bm * (n / bn)))
+  (wid : natlt (bm / (wm * tm) * (bn / (wn * tn))))
+  (mi : natlt wm)
+  (nj : natlt wn)
+= array2_subtile
+    (warp_tile (block_tile gD bm bn bid) (wm * tm) (wn * tn) wid)
+    tm tn mi nj
+
+let epilogue_chest
+  (#et_cd #et_acc : Type0)
+  {| scalar et_cd, scalar et_acc |}
+  (comb : et_cd -> et_acc -> et_cd)
+  (#rows #cols : nat)
+  (eC : chest2 et_cd rows cols)
+  (eAcc : chest2 et_acc rows cols)
+  : chest2 et_cd rows cols
+= mk2 (fun i j -> comb (acc2 eC i j) (acc2 eAcc i j))
+
+inline_for_extraction noextract
+fn epilogue_fragment_from_warp
+  (#et_cd #et_acc : Type0)
+  {| scd : scalar et_cd, real_like et_cd,
+     sacc : scalar et_acc, real_like et_acc |}
+  (comb : et_cd -> et_acc -> et_cd)
+  (comb_r : binop real { approx2 comb comb_r })
+  (#m #n : szp)
+  (c : array2 et_cd (rm m n))
+  (#_ : squash (SZ.fits (m * n)))
+  (bm bn rows cols wm wn : szp)
+  (#_ : squash (bm /?+ m /\ bn /?+ n /\
+                wm * rows /?+ bm /\ wn * cols /?+ bn))
+  (mrow : szlt (m / bm))
+  (mcol : szlt (n / bn))
+  (warpRow : szlt (bm / (wm * rows)))
+  (warpCol : szlt (bn / (wn * cols)))
+  (bid : szlt (m / bm * (n / bn)))
+  (wid : szlt (bm / (wm * rows) * (bn / (wn * cols))))
+  (#_ : squash (
+    SZ.v mrow == SZ.v bid / (SZ.v n / SZ.v bn) /\
+    SZ.v mcol == SZ.v bid % (SZ.v n / SZ.v bn) /\
+    SZ.v warpRow == SZ.v wid / (SZ.v bn / (SZ.v wn * SZ.v cols)) /\
+    SZ.v warpCol == SZ.v wid % (SZ.v bn / (SZ.v wn * SZ.v cols))))
+  (#fC : perm)
+  (#eC : chest2 et_cd m n)
+  (#rC : chest2 real m n)
+  (#_ : squash (eC %~ rC))
+  (#lAcc : layout2 rows cols) {| T.ctlayout lAcc |}
+  (acc : array2 et_acc lAcc)
+  (#eAcc : chest2 et_acc rows cols)
+  (#rAcc : chest2 real rows cols)
+  (#_ : squash (eAcc %~ rAcc))
+  (d : array2 et_cd (rm m n))
+  (idx : szlt (wm * wn))
+  (lane : szlt warp_size)
+  (#_ : squash (SZ.fits (rows * cols + warp_size)))
+  preserves
+    gpu **
+    c |-> Frac fC eC **
+    acc |-> Frac (1.0R /. warp_size) eAcc
+  requires
+    live_lane_cells
+      (output_fragment d bm bn rows cols wm wn
+        (SZ.v bid) (SZ.v wid) (SZ.v idx / wn) (SZ.v idx % wn))
+      lane
+  ensures
+    own_lane_cells
+      (output_fragment d bm bn rows cols wm wn
+        (SZ.v bid) (SZ.v wid) (SZ.v idx / wn) (SZ.v idx % wn))
+      (epilogue_chest comb
+        (ematrix_subtile
+          (ematrix_subtile
+            (ematrix_subtile eC bm bn (SZ.v mrow) (SZ.v mcol))
+            (wm * rows) (wn * cols) (SZ.v warpRow) (SZ.v warpCol))
+          rows cols (SZ.v idx / wn) (SZ.v idx % wn))
+        eAcc)
+      lane **
+    pure (
+      epilogue_chest comb
+        (ematrix_subtile
+          (ematrix_subtile
+            (ematrix_subtile eC bm bn (SZ.v mrow) (SZ.v mcol))
+            (wm * rows) (wn * cols) (SZ.v warpRow) (SZ.v warpCol))
+          rows cols (SZ.v idx / wn) (SZ.v idx % wn))
+        eAcc
+      %~
+      chest_comb comb_r
+        (ematrix_subtile
+          (ematrix_subtile
+            (ematrix_subtile rC bm bn (SZ.v mrow) (SZ.v mcol))
+            (wm * rows) (wn * cols) (SZ.v warpRow) (SZ.v warpCol))
+          rows cols (SZ.v idx / wn) (SZ.v idx % wn))
+        rAcc)
+
+inline_for_extraction noextract
+unfold let shmems_desc_to
+  (et_ab et_acc : Type0) {| sized et_ab, sized et_acc |}
+  (bm bn bk tm tn nthr : szp)
+  (#_ : squash (SZ.fits (bm * bk) /\ SZ.fits (bk * bn)))
+  (#_ : squash (SZ.fits ((nthr / warp_size) * tm * tn)))
+  (#_ : squash (warp_size /?+ nthr))
+  : list shmem_desc
+=
+  assert (SZ.fits ((nthr / warp_size) * tm));
+  [
+    SHArray et_ab (bm *^ bk);
+    SHArray et_ab (bk *^ bn);
+    SHArray et_acc ((nthr /^ warp_size) *^ tm *^ tn);
+  ]
+
+inline_for_extraction noextract
+let scratch_layout
+  (tm tn nthr : szp)
+  (#_ : squash (warp_size /?+ nthr))
+  : layout2 ((nthr / warp_size) * tm) tn
+= rm ((SZ.v nthr / warp_size) * SZ.v tm) (SZ.v tn)
+
+inline_for_extraction noextract
+let scratch_matrix
+  (#et_ab #et_acc : Type0)
+  {| sized et_ab, sized et_acc |}
+  (bm bn bk tm tn nthr : szp)
+  (#_ : squash (SZ.fits (bm * bk) /\ SZ.fits (bk * bn)))
+  (#_ : squash (SZ.fits ((nthr / warp_size) * tm * tn)))
+  (#_ : squash (warp_size /?+ nthr))
+  (sh : c_shmems (shmems_desc_to et_ab et_acc bm bn bk tm tn nthr))
+  : array2 et_acc (scratch_layout tm tn nthr)
+= from_array (scratch_layout tm tn nthr) (fst (snd (snd sh)))
+
+inline_for_extraction noextract
+let scratch_tile
+  (#et_ab #et_acc : Type0)
+  {| sized et_ab, sized et_acc |}
+  (bm bn bk tm tn nthr : szp)
+  (#_ : squash (SZ.fits (bm * bk) /\ SZ.fits (bk * bn)))
+  (#_ : squash (SZ.fits ((nthr / warp_size) * tm * tn)))
+  (#_ : squash (warp_size /?+ nthr))
+  (sh : c_shmems (shmems_desc_to et_ab et_acc bm bn bk tm tn nthr))
+  (wid : natlt (nthr / warp_size))
+= array2_subtile (scratch_matrix bm bn bk tm tn nthr sh)
+    (SZ.v tm) (SZ.v tn) wid 0
+
+inline_for_extraction noextract
+let scratch_tile_st
+  (#et_ab #et_acc : Type0)
+  {| sized et_ab, sized et_acc |}
+  (bm bn bk tm tn nthr : szp)
+  (#_ : squash (SZ.fits (bm * bk) /\ SZ.fits (bk * bn)))
+  (#_ : squash (SZ.fits ((nthr / warp_size) * tm * tn)))
+  (#_ : squash (warp_size /?+ nthr))
+  (sh : c_shmems (shmems_desc_to et_ab et_acc bm bn bk tm tn nthr))
+  (wid : szlt (nthr /^ warp_size))
+= scratch_tile bm bn bk tm tn nthr sh (SZ.v wid)
+
+let output_lane_live
+  (#et : Type0) {| scalar et |}
+  (#m #n : nat)
+  (gD : array2 et (rm m n))
+  (bm bn tm tn wm wn : pos)
+  (#_ : squash (bm /?+ m /\ bn /?+ n /\
+                wm * tm /?+ bm /\ wn * tn /?+ bn))
+  (bid : natlt (m / bm * (n / bn)))
+  (tid : natlt (bm / (wm * tm) * (bn / (wn * tn)) * warp_size))
+  : slprop
+= forall+ (mi : natlt wm) (nj : natlt wn).
+    live_lane_cells
+      (output_fragment gD bm bn tm tn wm wn bid (tid / warp_size) mi nj)
+      (tid % warp_size)
+
+let output_lane_approximates
+  (#et : Type0) {| scalar et, real_like et |}
+  (#m #n : nat)
+  (gD : array2 et (rm m n))
+  (bm bn tm tn wm wn : pos)
+  (#_ : squash (bm /?+ m /\ bn /?+ n /\
+                wm * tm /?+ bm /\ wn * tn /?+ bn))
+  (bid : natlt (m / bm * (n / bn)))
+  (tid : natlt (bm / (wm * tm) * (bn / (wn * tn)) * warp_size))
+  (rD : chest2 real (wm * tm) (wn * tn))
+  : slprop
+= forall+ (mi : natlt wm) (nj : natlt wn).
+    exists* (eD : chest2 et tm tn).
+      own_lane_cells
+        (output_fragment gD bm bn tm tn wm wn bid (tid / warp_size) mi nj)
+        eD
+        (tid % warp_size) **
+      pure (eD %~ ematrix_subtile rD tm tn mi nj)
+
+let scratch_tile_live
+  (#et_ab #et_acc : Type0)
+  {| sized et_ab, scalar et_acc |}
+  (bm bn bk tm tn nthr : szp)
+  (#_ : squash (SZ.fits (bm * bk) /\ SZ.fits (bk * bn)))
+  (#_ : squash (SZ.fits ((nthr / warp_size) * tm * tn)))
+  (#_ : squash (warp_size /?+ nthr))
+  (sh : c_shmems (shmems_desc_to et_ab et_acc bm bn bk tm tn nthr))
+  (tid : natlt nthr)
+  : slprop
+= exists* (eAcc : chest2 et_acc tm tn).
+    scratch_tile bm bn bk tm tn nthr sh (tid / warp_size)
+      |-> Frac (1.0R /. warp_size) eAcc
+
+unfold
+let kpre1_to
+  (#et_ab #et_cd : Type0)
+  {| scalar et_ab, real_like et_ab,
+     scalar et_cd, real_like et_cd |}
+  (#m #n #k : szp)
+  (#lA : layout2 m k)
+  (#lB : layout2 k n)
+  (gA : array2 et_ab lA)
+  (eA : chest2 et_ab m k)
+  (gB : array2 et_ab lB)
+  (eB : chest2 et_ab k n)
+  (gC : array2 et_cd (rm m n))
+  (eC : chest2 et_cd m n)
+  (gD : array2 et_cd (rm m n))
+  (bm bn bk tm tn tk wm wn : szp{
+    constraints bm bn bk tm tn tk wm wn})
+  (#_ : squash (bm /?+ m /\ bn /?+ n))
+  (fA fB fC : perm)
+  (rA : chest2 real m k)
+  (rB : chest2 real k n)
+  (rC : chest2 real m n)
+  (nblk : szp{SZ.v nblk == m / bm * (n / bn)})
+  (nthr : szp{
+    SZ.v nthr == bm / (wm * tm) * (bn / (wn * tn)) * warp_size})
+  (bid : natlt nblk)
+  (tid : natlt nthr)
+  : slprop
+= gA |-> Frac (fA /. (nblk * nthr)) eA **
+  gB |-> Frac (fB /. (nblk * nthr)) eB **
+  gC |-> Frac (fC /. (nblk * nthr)) eC **
+  output_lane_live gD bm bn tm tn wm wn bid tid **
+  pure (aligned 16 (core gA)) **
+  pure (aligned 16 (core gB)) **
+  pure (eA %~ rA) **
+  pure (eB %~ rB) **
+  pure (eC %~ rC)
+
+unfold
+let kpost1_to
+  (#et_ab #et_cd : Type0)
+  {| scalar et_ab, scalar et_cd, real_like et_cd |}
+  (comb_r : binop real)
+  (#m #n #k : szp)
+  (#lA : layout2 m k)
+  (#lB : layout2 k n)
+  (gA : array2 et_ab lA)
+  (eA : chest2 et_ab m k)
+  (gB : array2 et_ab lB)
+  (eB : chest2 et_ab k n)
+  (gC : array2 et_cd (rm m n))
+  (eC : chest2 et_cd m n)
+  (gD : array2 et_cd (rm m n))
+  (bm bn bk tm tn tk wm wn : szp{
+    constraints bm bn bk tm tn tk wm wn})
+  (#_ : squash (bm /?+ m /\ bn /?+ n))
+  (fA fB fC : perm)
+  (rA : chest2 real m k)
+  (rB : chest2 real k n)
+  (rC : chest2 real m n)
+  (nblk : szp{SZ.v nblk == m / bm * (n / bn)})
+  (nthr : szp{
+    SZ.v nthr == bm / (wm * tm) * (bn / (wn * tn)) * warp_size})
+  (bid : natlt nblk)
+  (tid : natlt nthr)
+  : slprop
+= gA |-> Frac (fA /. (nblk * nthr)) eA **
+  gB |-> Frac (fB /. (nblk * nthr)) eB **
+  gC |-> Frac (fC /. (nblk * nthr)) eC **
+  output_lane_approximates
+    gD bm bn tm tn wm wn bid tid
+    (ematrix_subtile
+      (ematrix_subtile
+        (MS.mmcomb comb_r rC rA rB)
+        bm bn
+        (bid / (n / bn))
+        (bid % (n / bn)))
+      (wm * tm) (wn * tn)
+      ((tid / warp_size) / (bn / (wn * tn)))
+      ((tid / warp_size) % (bn / (wn * tn))))
+
+let shared_thread_live
+  (#et_ab #et_acc : Type0)
+  {| scalar et_ab, scalar et_acc |}
+  (bm bn bk tm tn nthr : szp)
+  (#_ : squash (SZ.fits (bm * bk) /\ SZ.fits (bk * bn)))
+  (#_ : squash (SZ.fits ((nthr / warp_size) * tm * tn)))
+  (#_ : squash (warp_size /?+ nthr))
+  (sh : c_shmems (shmems_desc_to et_ab et_acc bm bn bk tm tn nthr))
+  (tid : natlt nthr)
+  : slprop
+= live_c_shmem (fst sh) #(1.0R /. nthr) **
+  live_c_shmem (fst (snd sh)) #(1.0R /. nthr) **
+  scratch_tile_live bm bn bk tm tn nthr sh tid
+
+unfold
+let kpre_to
+  (#et_ab #et_cd #et_acc : Type0)
+  {| scalar et_ab, real_like et_ab,
+     scalar et_cd, real_like et_cd, scalar et_acc |}
+  (#m #n #k : szp)
+  (#lA : layout2 m k)
+  (#lB : layout2 k n)
+  (gA : array2 et_ab lA)
+  (eA : chest2 et_ab m k)
+  (gB : array2 et_ab lB)
+  (eB : chest2 et_ab k n)
+  (gC : array2 et_cd (rm m n))
+  (eC : chest2 et_cd m n)
+  (gD : array2 et_cd (rm m n))
+  (bm bn bk tm tn tk wm wn : szp{
+    constraints bm bn bk tm tn tk wm wn})
+  (#_ : squash (bm /?+ m /\ bn /?+ n))
+  (#_ : squash (SZ.fits (bm * bk) /\ SZ.fits (bk * bn)))
+  (#_ : squash (SZ.fits (
+    ((bm / (wm * tm) * (bn / (wn * tn)) * warp_size) / warp_size)
+      * tm * tn)))
+  (#_ : squash (
+    warp_size /?+ (bm / (wm * tm) * (bn / (wn * tn)) * warp_size)))
+  (fA fB fC : perm)
+  (rA : chest2 real m k)
+  (rB : chest2 real k n)
+  (rC : chest2 real m n)
+  (nblk : szp{SZ.v nblk == m / bm * (n / bn)})
+  (nthr : szp{
+    SZ.v nthr == bm / (wm * tm) * (bn / (wn * tn)) * warp_size})
+  (sh : c_shmems (shmems_desc_to et_ab et_acc bm bn bk tm tn nthr))
+  (bid : natlt nblk)
+  (tid : natlt nthr)
+  : slprop
+= kpre1_to gA eA gB eB gC eC gD
+    bm bn bk tm tn tk wm wn fA fB fC rA rB rC nblk nthr bid tid **
+  shared_thread_live bm bn bk tm tn nthr sh tid
+
+unfold
+let kpost_to
+  (#et_ab #et_cd #et_acc : Type0)
+  {| scalar et_ab, scalar et_cd, real_like et_cd, scalar et_acc |}
+  (comb_r : binop real)
+  (#m #n #k : szp)
+  (#lA : layout2 m k)
+  (#lB : layout2 k n)
+  (gA : array2 et_ab lA)
+  (eA : chest2 et_ab m k)
+  (gB : array2 et_ab lB)
+  (eB : chest2 et_ab k n)
+  (gC : array2 et_cd (rm m n))
+  (eC : chest2 et_cd m n)
+  (gD : array2 et_cd (rm m n))
+  (bm bn bk tm tn tk wm wn : szp{
+    constraints bm bn bk tm tn tk wm wn})
+  (#_ : squash (bm /?+ m /\ bn /?+ n))
+  (#_ : squash (SZ.fits (bm * bk) /\ SZ.fits (bk * bn)))
+  (#_ : squash (SZ.fits (
+    ((bm / (wm * tm) * (bn / (wn * tn)) * warp_size) / warp_size)
+      * tm * tn)))
+  (#_ : squash (
+    warp_size /?+ (bm / (wm * tm) * (bn / (wn * tn)) * warp_size)))
+  (fA fB fC : perm)
+  (rA : chest2 real m k)
+  (rB : chest2 real k n)
+  (rC : chest2 real m n)
+  (nblk : szp{SZ.v nblk == m / bm * (n / bn)})
+  (nthr : szp{
+    SZ.v nthr == bm / (wm * tm) * (bn / (wn * tn)) * warp_size})
+  (sh : c_shmems (shmems_desc_to et_ab et_acc bm bn bk tm tn nthr))
+  (bid : natlt nblk)
+  (tid : natlt nthr)
+  : slprop
+= kpost1_to comb_r gA eA gB eB gC eC gD
+    bm bn bk tm tn tk wm wn fA fB fC rA rB rC nblk nthr bid tid **
+  shared_thread_live bm bn bk tm tn nthr sh tid
+
+ghost
+fn setup_to
+  (#et_ab #et_cd : Type0)
+  {| scalar et_ab, real_like et_ab,
+     scalar et_cd, real_like et_cd |}
+  (#m #n #k : szp)
+  (#lA : layout2 m k)
+  (#lB : layout2 k n)
+  (gA : array2 et_ab lA)
+  (eA : chest2 et_ab m k)
+  (gB : array2 et_ab lB)
+  (eB : chest2 et_ab k n)
+  (#_ : squash (aligned 16 (core gA)))
+  (#_ : squash (aligned 16 (core gB)))
+  (gC : array2 et_cd (rm m n))
+  (eC : chest2 et_cd m n)
+  (gD : array2 et_cd (rm m n))
+  (#_ : squash (SZ.fits (m * n)))
+  (bm bn bk tm tn tk wm wn : szp{
+    constraints bm bn bk tm tn tk wm wn})
+  (#_ : squash (bm /?+ m /\ bn /?+ n))
+  (nblk : szp{SZ.v nblk == m / bm * (n / bn)})
+  (nthr : szp{
+    SZ.v nthr == bm / (wm * tm) * (bn / (wn * tn)) * warp_size})
+  (fA fB fC : perm)
+  (rA : chest2 real m k)
+  (rB : chest2 real k n)
+  (rC : chest2 real m n)
+  ()
+  norewrite
+  requires
+    gA |-> Frac fA eA ** pure (eA %~ rA) **
+    gB |-> Frac fB eB ** pure (eB %~ rB) **
+    gC |-> Frac fC eC ** pure (eC %~ rC) **
+    live gD
+  ensures
+    (forall+ (bid : natlt nblk) (tid : natlt nthr).
+      kpre1_to gA eA gB eB gC eC gD
+        bm bn bk tm tn tk wm wn fA fB fC rA rB rC
+        nblk nthr bid tid) **
+    pure (SZ.fits ((rm m n).ulen))
+
+ghost
+fn block_setup_to
+  (#et_ab #et_cd #et_acc : Type0)
+  {| scalar et_ab, real_like et_ab,
+     scalar et_cd, real_like et_cd, scalar et_acc |}
+  (#m #n #k : szp)
+  (#lA : layout2 m k)
+  (#lB : layout2 k n)
+  (gA : array2 et_ab lA)
+  (eA : chest2 et_ab m k)
+  (gB : array2 et_ab lB)
+  (eB : chest2 et_ab k n)
+  (gC : array2 et_cd (rm m n))
+  (eC : chest2 et_cd m n)
+  (gD : array2 et_cd (rm m n))
+  (bm bn bk tm tn tk wm wn : szp{
+    constraints bm bn bk tm tn tk wm wn})
+  (#_ : squash (bm /?+ m /\ bn /?+ n))
+  (#_ : squash (SZ.fits (bm * bk) /\ SZ.fits (bk * bn)))
+  (#_ : squash (SZ.fits (
+    ((bm / (wm * tm) * (bn / (wn * tn)) * warp_size) / warp_size)
+      * tm * tn)))
+  (#_ : squash (
+    warp_size /?+ (bm / (wm * tm) * (bn / (wn * tn)) * warp_size)))
+  (fA fB fC : perm)
+  (rA : chest2 real m k)
+  (rB : chest2 real k n)
+  (rC : chest2 real m n)
+  (nblk : szp{SZ.v nblk == m / bm * (n / bn)})
+  (nthr : szp{
+    SZ.v nthr == bm / (wm * tm) * (bn / (wn * tn)) * warp_size})
+  (sh : c_shmems (shmems_desc_to et_ab et_acc bm bn bk tm tn nthr))
+  (bid : natlt nblk)
+  ()
+  norewrite
+  requires
+    live_c_shmems sh **
+    (forall+ (tid : natlt nthr).
+      kpre1_to gA eA gB eB gC eC gD
+        bm bn bk tm tn tk wm wn fA fB fC rA rB rC
+        nblk nthr bid tid)
+  ensures
+    (forall+ (tid : natlt nthr).
+      kpre_to gA eA gB eB gC eC gD
+        bm bn bk tm tn tk wm wn fA fB fC rA rB rC
+        nblk nthr sh bid tid) **
+    emp
+
+ghost
+fn block_teardown_to
+  (#et_ab #et_cd #et_acc : Type0)
+  {| scalar et_ab, scalar et_cd, real_like et_cd, scalar et_acc |}
+  (comb_r : binop real)
+  (#m #n #k : szp)
+  (#lA : layout2 m k)
+  (#lB : layout2 k n)
+  (gA : array2 et_ab lA)
+  (eA : chest2 et_ab m k)
+  (gB : array2 et_ab lB)
+  (eB : chest2 et_ab k n)
+  (gC : array2 et_cd (rm m n))
+  (eC : chest2 et_cd m n)
+  (gD : array2 et_cd (rm m n))
+  (bm bn bk tm tn tk wm wn : szp{
+    constraints bm bn bk tm tn tk wm wn})
+  (#_ : squash (bm /?+ m /\ bn /?+ n))
+  (#_ : squash (SZ.fits (bm * bk) /\ SZ.fits (bk * bn)))
+  (#_ : squash (SZ.fits (
+    ((bm / (wm * tm) * (bn / (wn * tn)) * warp_size) / warp_size)
+      * tm * tn)))
+  (#_ : squash (
+    warp_size /?+ (bm / (wm * tm) * (bn / (wn * tn)) * warp_size)))
+  (fA fB fC : perm)
+  (rA : chest2 real m k)
+  (rB : chest2 real k n)
+  (rC : chest2 real m n)
+  (nblk : szp{SZ.v nblk == m / bm * (n / bn)})
+  (nthr : szp{
+    SZ.v nthr == bm / (wm * tm) * (bn / (wn * tn)) * warp_size})
+  (sh : c_shmems (shmems_desc_to et_ab et_acc bm bn bk tm tn nthr))
+  (bid : natlt nblk)
+  ()
+  norewrite
+  requires
+    (forall+ (tid : natlt nthr).
+      kpost_to comb_r gA eA gB eB gC eC gD
+        bm bn bk tm tn tk wm wn fA fB fC rA rB rC
+        nblk nthr sh bid tid) **
+    emp
+  ensures
+    live_c_shmems sh **
+    (forall+ (tid : natlt nthr).
+      kpost1_to comb_r gA eA gB eB gC eC gD
+        bm bn bk tm tn tk wm wn fA fB fC rA rB rC
+        nblk nthr bid tid)
+
+ghost
+fn teardown_to
+  (#et_ab #et_cd : Type0)
+  {| scalar et_ab, scalar et_cd, real_like et_cd |}
+  (comb_r : binop real)
+  (#m #n #k : szp)
+  (#lA : layout2 m k)
+  (#lB : layout2 k n)
+  (gA : array2 et_ab lA)
+  (eA : chest2 et_ab m k)
+  (gB : array2 et_ab lB)
+  (eB : chest2 et_ab k n)
+  (gC : array2 et_cd (rm m n))
+  (eC : chest2 et_cd m n)
+  (gD : array2 et_cd (rm m n))
+  (#_ : squash (SZ.fits (m * n)))
+  (bm bn bk tm tn tk wm wn : szp{
+    constraints bm bn bk tm tn tk wm wn})
+  (#_ : squash (bm /?+ m /\ bn /?+ n))
+  (nblk : szp{SZ.v nblk == m / bm * (n / bn)})
+  (nthr : szp{
+    SZ.v nthr == bm / (wm * tm) * (bn / (wn * tn)) * warp_size})
+  (fA fB fC : perm)
+  (rA : chest2 real m k)
+  (rB : chest2 real k n)
+  (rC : chest2 real m n)
+  ()
+  norewrite
+  requires
+    (forall+ (bid : natlt nblk) (tid : natlt nthr).
+      kpost1_to comb_r gA eA gB eB gC eC gD
+        bm bn bk tm tn tk wm wn fA fB fC rA rB rC
+        nblk nthr bid tid) **
+    pure (SZ.fits ((rm m n).ulen))
+  ensures
+    gA |-> Frac fA eA **
+    gB |-> Frac fB eB **
+    gC |-> Frac fC eC **
+    (exists* (eD : chest2 et_cd m n).
+      gD |-> eD ** pure (eD %~ MS.mmcomb comb_r rC rA rB))
